@prefix schema: <http://schema.org/> .
@prefix rdfs: <http://www.w3.org/2000/01/rdf-schema#> .
@prefix dc: <http://purl.org/dc/terms/> .
@prefix rdf: <http://www.w3.org/1999/02/22-rdf-syntax-ns#> .

schema:ChemicalSubstance
  a rdfs:Class ;
  schema:isPartOf <http://bio.schema.org> ;
  rdfs:label "ChemicalSubstance" ;
  rdfs:comment "A chemical substance is 'a portion of matter of constant composition, composed of molecular entities of the same type or of different types' (source: [ChEBI:59999](https://www.ebi.ac.uk/chebi/searchId.do?chebiId=59999))." ;
  rdfs:subClassOf schema:BioChemEntity ;
  dc:source <http://bioschemas.org>, <https://www.ebi.ac.uk/chebi/searchId.do?chebiId=59999> .

schema:chemicalComposition
  a rdf:Property ;
  schema:isPartOf <http://bio.schema.org> ;
  rdfs:label "chemicalComposition" ;
  rdfs:comment "The chemical composition describes the identity and relative ratio of the chemical elements that make up the substance." ;
  schema:domainIncludes schema:ChemicalSubstance ;
  schema:rangeIncludes schema:Text ;
  dc:source <http://www.bioschemas.org/ChemicalSubstance> .

schema:chemicalRole
  a rdf:Property ;
  schema:isPartOf <http://bio.schema.org> ;
  rdfs:label "chemicalRole" ;
  rdfs:comment "A role played by the BioChemEntity within a chemical context." ;
  schema:domainIncludes schema:ChemicalSubstance, schema:MolecularEntity ;
  schema:rangeIncludes schema:DefinedTerm ;
  dc:source <http://www.bioschemas.org/ChemicalSubstance> .

schema:potentialUse
  a rdf:Property ;
  schema:isPartOf <http://bio.schema.org> ;
  rdfs:label "potentialUse" ;
  rdfs:comment "Intended use of the BioChemEntity by humans." ;
  schema:domainIncludes schema:ChemicalSubstance, schema:MolecularEntity ;
  schema:rangeIncludes schema:DefinedTerm ;
  dc:source <http://www.bioschemas.org/ChemicalSubstance> .
